update interface

code/aes/Hacl.Impl.AES.SubBytes.fst
@@ -3,12 +3,12 @@ friend Lib.Sequence
 friend Lib.LoopCombinators
 friend FStar.Seq.Base
 
-open FStar.HyperStack.ST
-open FStar.HyperStack
-
-module IT = Lib.IntTypes
 module B = Lib.Buffer
+module IT = Lib.IntTypes
 module S = Lib.Sliceable
+
+open FStar.HyperStack
+open FStar.HyperStack.ST
 
 #set-options "--fuel 1 --ifuel 1"
 
@@ -98,7 +98,7 @@ match i with
 | 7 -> 111
 
 inline_for_extraction noextract
-let sub_bytes_spec (#n:IT.size_nat) (#xN:S.sig n) (x:S.xNxM xN 8) : S.xNxM xN 8 =
+let sub_bytes_spec #n #xN x =
   S.reduce_output (S.circuit_spec circ) 8 circ_outputs x
 
 open FStar.Tactics
@@ -122,23 +122,9 @@ let sub_bytes_spec_theorem (#n:IT.size_nat) (#xN:S.sig n) (x:S.xNxM xN 8) (j:nat
   =
   sub_bytes_bruteforce_lemma ()
 
-inline_for_extraction noextract
-private let u64 = S.uN IT.U64 IT.SEC
-
 
 #push-options "--fuel 0 --ifuel 0 --z3rlimit 20"
-let sub_bytes64x8
-  (st0:u64.t) (st1:u64.t) (st2:u64.t) (st3:u64.t)
-  (st4:u64.t) (st5:u64.t) (st6:u64.t) (st7:u64.t) :
-    Stack
-      (u64.t * u64.t * u64.t * u64.t * u64.t * u64.t * u64.t * u64.t)
-      (fun _ -> True)
-      (fun h0 (o0,o1,o2,o3,o4,o5,o6,o7) h1 ->
-        B.modifies LowStar.Monotonic.Buffer.loc_none h0 h1
-        /\ S.uNx8_mk o0 o1 o2 o3 o4 o5 o6 o7
-          == sub_bytes_spec (S.uNx8_mk st0 st1 st2 st3 st4 st5 st6 st7)
-      )
-  =
+let sub_bytes64x8 st0 st1 st2 st3 st4 st5 st6 st7 =
   push_frame();
   let input : B.lbuffer u64.t 8ul = B.create _ u64.zeros_ in
   B.create8 input st0 st1 st2 st3 st4 st5 st6 st7;
